Clean Array theory.
Word should be based off of this with fixed length and base type.

theories/datatypes/Array.ec
@@ -5,633 +5,157 @@
  * Distributed under the terms of the CeCILL-B-V1 license
  * -------------------------------------------------------------------- *)
 
-(* A theory of polymorphic arrays. *)
+(* -------------------------------------------------------------------- *)
+require import Option Logic Fun Int List.
 
-(*
- * All operators are only partially specified, as we may choose to match
- * them with various programming language constructs.
- * 
- * The user wanting to instantiate it with particular implementation
- * choices should clone it and add axioms to further refine the
- * operators.
- *
- * The operator names for imperative operators correspond to the OCaml Array library.
- *
- *)
+(* -------------------------------------------------------------------- *)
+type 'a array.
 
-require import Logic Fun Int IntExtra.
+op mkarray : 'a list -> 'a array.
+op ofarray : 'a array -> 'a list.
 
-(*********************************)
-(*             Core              *)
-(*********************************)
-(* A type *)
-type 'x array.
+axiom nosmt mkarrayK : cancel ofarray<:'a> mkarray.
+axiom nosmt ofarrayK : cancel mkarray<:'a> ofarray.
 
-(* Arrays have a non-negative length *)
-op length: 'x array -> int.
-axiom length_pos: forall (xs:'x array), 0 <= length xs.
+lemma nosmt arrayW (P : 'a array -> bool):
+     (forall s, P (mkarray s))
+  => forall n, P n.
+proof. by move=> ih n; rewrite -mkarrayK; apply/ih. qed.
 
-op "`|_|" (xs:'x array) = length xs.
+lemma nosmt mkarray_inj: injective mkarray<:'a>.
+proof. by apply/(can_inj _ _ ofarrayK). qed.
 
-(* And a bunch of elements *)
-op "_.[_]": 'x array -> int -> 'x.
+lemma nosmt ofarray_inj: injective ofarray<:'a>.
+proof. by apply/(can_inj _ _ mkarrayK). qed.
 
-(* Equality is extensional *)
-pred (==) (xs0 xs1:'x array) =
-  length xs0 = length xs1 /\
-  forall (i:int), 0 <= i < length xs0 => xs0.[i] = xs1.[i].
+(* -------------------------------------------------------------------- *)
+op size (arr : 'a array) = size (ofarray arr)
+axiomatized by sizeE.
 
-axiom array_ext (xs0 xs1:'x array):
-  xs0 == xs1 => xs0 = xs1.
+op "_.[_]" (arr : 'a array) (i : int) = nth witness (ofarray arr) i
+axiomatized by getE.
 
-lemma rw_array_ext (xs0 xs1:'x array):
-  xs0 == xs1 <=> xs0 = xs1.
-proof strict.
-by split; first apply array_ext.
+op "_.[_<-_]" (arr : 'a array) (i : int) (x : 'a) =
+  mkarray (mkseq (fun k => if i = k then x else arr.[k]) (size arr))
+axiomatized by setE.
+
+(* -------------------------------------------------------------------- *)
+lemma size_ge0 (arr : 'a array): 0 <= size arr.
+proof. by rewrite sizeE size_ge0. qed.
+
+lemma size_mkarray (s : 'a list): size (mkarray s) = size s.
+proof. by rewrite sizeE ofarrayK. qed.
+
+(* -------------------------------------------------------------------- *)
+(* FIXME: name scheme copied from List.nth. It looks ridiculous. *)
+lemma nosmt get_neg (arr : 'a array) (i : int):
+  i < 0 => arr.[i] = witness.
+proof. by rewrite getE; apply/nth_neg. qed.
+
+lemma nosmt get_default (arr : 'a array) (i : int):
+  size arr <= i => arr.[i] = witness.
+proof. rewrite getE sizeE; apply/nth_default. qed.
+
+lemma nosmt arrayP (arr1 arr2 : 'a array):
+  (   size arr1 = size arr2
+   /\ (forall i, 0 <= i < size arr1 => arr1.[i] = arr2.[i]))
+  <=> arr1 = arr2.
+proof.
+split=> [[size_eq eq_get]|->//].
+apply/ofarray_inj/(eq_from_nth witness)=> [|i]; rewrite -!sizeE//.
++ by rewrite -!getE=> /eq_get.
 qed.
 
-(*********************************)
-(*    "Functional" Operators     *)
-(*********************************)
-(* Using these should be avoided when extracting,
-   for performance reasons. *)
-(* empty *)
-op empty: 'x array.
-
-axiom length_empty: length (empty<:'x>) = 0.
-
-lemma empty_unique (xs:'x array):
-  length(xs) = 0 => xs = empty.
-proof strict.
-by intros=> xs_0; apply array_ext; split;
-     [rewrite length_empty | smt].
+(* -------------------------------------------------------------------- *)
+lemma get_set_if (arr : 'a array) (x : 'a) (i j : int):
+  arr.[i <- x].[j] = if 0 <= i < size arr /\ j = i then x else arr.[j].
+proof.
+elim/arrayW: arr=> arr; rewrite !(setE, getE, size_mkarray, ofarrayK).
+rewrite nth_mkseq_if (eq_sym j).
+case: (0 <= j < size arr)=> [|^j_out /(nth_out witness) ->].
++ by case: (i = j)=> //= [-> -> //|]; rewrite getE ofarrayK.
++ by case: (i = j)=> [->|//=]; rewrite j_out.
 qed.
 
-(* cons *)
-op (::) : 'x -> 'x array -> 'x array.
+(* -------------------------------------------------------------------- *)
+lemma get_set (arr : 'a array) (x : 'a) (i j : int): 0 <= i < size arr =>
+  arr.[i <- x].[j] = if j = i then x else arr.[j].
+proof. by move=> lt_in; rewrite get_set_if lt_in. qed.
 
-axiom length_cons (x:'x) (xs:'x array):
-  length (x::xs) = 1 + length xs.
-
-axiom get_cons (x:'x) (xs:'x array) (i:int):
-  0 <= i <= length xs =>
-  (x::xs).[i] = (0 = i) ? x : xs.[i - 1].
-
-lemma cons_nonempty (x:'x) (xs:'x array):
-  x::xs <> empty.
-proof strict.
-by rewrite -not_def=> cons_empty;
-   cut:= congr1 length (x::xs) empty _=> //;
-   rewrite length_empty length_cons; smt.
+(* -------------------------------------------------------------------- *)
+lemma size_set (arr : 'a array) (x : 'a) (i : int):
+  size arr.[i <- x] = size arr.
+proof.
+rewrite setE size_mkarray size_mkseq /max.
+by have /lez_eqVlt [->//=|->//=]:= size_ge0 arr.
 qed.
 
-lemma consI (x y:'x) (xs ys:'x array):
-  x::xs = y::ys <=> x = y /\ xs = ys.
-proof strict.
-split; last by intros=> [-> ->].
-rewrite - !rw_array_ext /(==)=> [len val].
-do !split.
-  cut:= val 0 _; first smt.
-  by rewrite 2?get_cons /=; first 2 smt.
-  by generalize len; rewrite 2!length_cons; smt.
-  intros=> i i_bnd; cut := val (i + 1) _; first smt.
-  rewrite 2?get_cons; first 2 smt.
-  cut ->: (0 = i + 1) = false by smt.
-  cut ->: i + 1 - 1 = i by smt.
-  smt.
+(* -------------------------------------------------------------------- *)
+lemma set_out (i : int) (x : 'a) (arr : 'a array):
+  ! (0 <= i < size arr) => arr.[i <- x] = arr.
+proof.
+move=> Nlt_in; apply/arrayP; rewrite size_set//=.
+by move=> j; rewrite get_set_if Nlt_in.
 qed.
 
-(* snoc *)
-op (:::): 'x array -> 'x -> 'x array.
+(* -------------------------------------------------------------------- *)
+lemma set_neg (i : int) (a : 'a) (arr : 'a array):
+  i < 0 => arr.[i<- a] = arr.
+proof. by move=> lt0_i; rewrite set_out // lezNgt lt0_i. qed.
 
-axiom length_snoc (x:'x) (xs:'x array):
-  length (xs:::x) = length xs + 1.
+(* -------------------------------------------------------------------- *)
+lemma set_above (i : int) (a : 'a) (arr : 'a array):
+  size arr <= i => arr.[i <- a] = arr.
+proof. by move=> le_ni; rewrite set_out // ltzNge le_ni. qed.
 
-axiom get_snoc (xs:'x array) (x:'x) (i:int):
-  0 <= i <= length xs =>
-  (xs:::x).[i] = (i < length xs) ? xs.[i] : x.
-
-lemma snoc_nonempty (xs:'x array, x:'x):
-  xs:::x <> empty.
-proof strict.
-by rewrite -not_def=> snoc_empty;
-   cut:= congr1 length (xs:::x) empty _=> //;
-   rewrite length_empty length_snoc; smt.
+(* -------------------------------------------------------------------- *)
+lemma set_set_if (arr : 'a array) (k k' : int) (x x' : 'a):
+       arr.[k <- x].[k' <- x']
+    =  if   k = k'
+       then arr.[k' <- x']
+       else arr.[k' <- x'].[k <- x].
+proof.
+apply/arrayP; split; rewrite !size_set.
+  by rewrite fun_if; rewrite !size_set if_same.
+move=> i lt_in; case: (0 <= k < size arr)=> [lt_ksz|]; last first.
+  by move=> ?; rewrite !(set_out k) ?size_set.
+case: (0 <= k' < size arr)=> [lt_k'sz|]; last first.
+  by move=> ?; rewrite !(set_out k') ?size_set //; case: (k = k').
+rewrite fun_if2; rewrite !get_set ?size_set //.
+case: (k = k') => [->>|]; first by case: (i = k').
+by case: (i = k') => //; case: (i = k).
 qed.
 
-(* Induction Principle *)
-axiom array_ind (p:'x array -> bool):
-  p empty =>
-  (forall x xs, p xs => p (x::xs)) =>
-  (forall xs, p xs).
+(* -------------------------------------------------------------------- *)
+lemma set_set_eq (arr : 'a array) (k : int) (x x' : 'a):
+  arr.[k <- x].[k <- x'] = arr.[k <- x'].
+proof. by rewrite set_set_if. qed.
 
-(***************************)
-(*      OCaml Arrays       *)
-(***************************)
-(* set *)
-op "_.[_<-_]": 'x array -> int -> 'x -> 'x array.
+(* -------------------------------------------------------------------- *)
+lemma set_set_swap (arr : 'a array) (k k' : int) (x x' : 'a):
+  k <> k => arr.[k <- x].[k' <- x'] = arr.[k' <- x'].[k' <- x'].
+proof. by rewrite set_set_if. qed.
 
-axiom length_set (i:int) (x:'x) (xs:'x array):
-  length (xs.[i <- x]) = length xs.
+(* -------------------------------------------------------------------- *)
+op offun f n: 'a array = mkarray (mkseq f n).
 
-axiom get_set (xs:'x array) (i j:int) (x:'x):
-  0 <= j < length xs =>
-  xs.[i <- x].[j] = (i = j) ? x : xs.[j].
+lemma offunifE (f : int -> 'a) n i:
+  (offun f n).[i] = if 0 <= i < n then f i else witness.
+proof. by rewrite getE ofarrayK nth_mkseq_if. qed.
 
-lemma set_set i j (x y:'x) xs:
-  xs.[i <- x].[j <- y] =
-    (i = j) ? xs.[j <- y] :
-              xs.[j <- y].[i <- x].
-proof strict.
-by apply array_ext; split; smt.
+lemma offunE n (f : int -> 'a) i: 0 <= i < n => (offun f n).[i] = f i.
+proof. by move=> lt_in; rewrite offunifE lt_in. qed.
+
+lemma size_offun (f : int -> 'a) n: size (offun f n) = max 0 n.
+proof. by rewrite size_mkarray size_mkseq. qed.
+
+(* -------------------------------------------------------------------- *)
+op map (f : 'a -> 'b) (arr : 'a array) : 'b array =
+  mkarray (map f (ofarray arr)).
+
+lemma mapE (f : 'a -> 'b) arr i: 0 <= i < size arr =>
+  (map f arr).[i] = f arr.[i].
+proof.
+elim/arrayW: arr => arr; rewrite size_mkarray !getE !ofarrayK.
+by apply/nth_map.
 qed.
-
-lemma nosmt set_setE x i (y:'a) xs:
-  xs.[i <- x].[i <- y] = xs.[i <- y].
-proof strict.
-by rewrite set_set.
-qed.
-
-lemma nosmt set_setN x i j (y:'a) xs:
-  i <> j =>
-  xs.[i <- x].[j <- y] = xs.[j <- y].[i <- x].
-proof strict.
-by rewrite set_set -neqF=> ->.
-qed.
-
-(* make *)
-op make: int -> 'x -> 'x array.
-
-axiom length_make (x:'x) l:
-  0 <= l =>
-  length (make l x) = l.
-
-axiom get_make l (x:'x) i:
-  0 <= i < l =>
-  (make l x).[i] = x.
-
-(* init *)
-op init: int -> (int -> 'x) -> 'x array.
-
-axiom length_init (f:int -> 'x) l:
-  0 <= l =>
-  length (init l f) = l.
-
-axiom get_init l (f:int -> 'x) i:
-  0 <= i < l =>
-  (init l f).[i] = f i.
-
-axiom nosmt make_init n (a:'a) : init n (fun x, a) = make n a.
-
-(* append *)
-op (||): 'x array -> 'x array -> 'x array.
-
-axiom length_append (xs0 xs1:'x array):
-  length (xs0 || xs1) = length xs0 + length xs1.
-
-axiom get_append (xs0 xs1:'x array) (i:int):
-  0 <= i < length (xs0 || xs1) =>
-  (xs0 || xs1).[i] = (0 <= i < length xs0) ? xs0.[i] : xs1.[i - length xs0].
-
-lemma nosmt get_append_left (xs0 xs1:'x array) (i:int):
- 0 <= i < length xs0 =>
- (xs0 || xs1).[i] = xs0.[i]
-by smt.
-
-lemma nosmt get_append_right (xs0 xs1:'x array) (i:int):
- length xs0 <= i < length xs0 + length xs1 =>
- (xs0 || xs1).[i] = xs1.[i - length xs0]
-by smt.
-
-axiom set_append (xs0 xs1:'x array) (i:int) v:
-  0 <= i < length (xs0 || xs1) =>
-  (xs0 || xs1).[i <- v] = (0 <= i < length xs0) ? 
-     (xs0.[i <- v] || xs1) : (xs0 || xs1.[i - length xs0 <- v]).
-
-lemma nosmt set_append_left (xs0 xs1:'x array) (i:int) v:
- 0 <= i < length xs0 =>
- (xs0 || xs1).[i <- v] = (xs0.[i <- v] || xs1)
-by smt.
-
-lemma nosmt set_append_right (xs0 xs1:'x array) (i:int) v:
- length xs0 <= i < length xs0 + length xs1 =>
- (xs0 || xs1).[i <- v] = (xs0 || xs1.[i - length xs0 <- v])
-by smt.
-
-lemma make_append (a:'a) (l1 l2:int):
-  0 <= l1 => 0 <= l2 => make (l1 + l2) a = (make l1 a || make l2 a).
-proof. move=> le0_l1 le0_l2; apply/array_ext; smt. qed.
-
-(* sub *)
-op sub: 'x array -> int -> int -> 'x array.
-
-axiom length_sub (xs:'x array) (s l:int):
-  0 <= s => 0 <= l => s + l <= length xs =>
-  length (sub xs s l) = l.
-
-axiom get_sub (xs:'x array) (s l i:int):
-  0 <= s => 0 <= l => s + l <= length xs =>
-  0 <= i < l =>
-  (sub xs s l).[i] = xs.[i + s].
-
-(* fill *)
-op fill: 'x array -> int -> int -> 'x -> 'x array.
-
-axiom length_fill (s l:int) x (xs:'x array):
-  0 <= s => 0 <= l => s + l <= length xs =>
-  length (fill xs s l x) = length xs.
-
-axiom get_fill (xs:'x array) (s l:int) x i:
-  0 <= s => 0 <= l => s + l <= length xs =>
-  0 <= i < length xs =>
-  (fill xs s l x).[i] = (s <= i < s + l) ? x : xs.[i].
-
-(* blit (previously write) *)
-op blit: 'x array -> int -> 'x array -> int -> int -> 'x array.
-
-axiom length_blit (dst src:'x array) (dOff sOff l:int):
-  0 <= dOff => 0 <= sOff => 0 <= l =>
-  dOff + l <= length dst =>
-  sOff + l <= length src =>
-  length (blit dst dOff src sOff l) = length dst.
-
-axiom get_blit (dst src:'x array) (dOff sOff l i:int):
-  0 <= dOff => 0 <= sOff => 0 <= l =>
-  dOff + l <= length dst =>
-  sOff + l <= length src =>
-  0 <= i < length dst =>
-  (blit dst dOff src sOff l).[i] =
-    (dOff <= i < dOff + l) ? src.[i - dOff + sOff]
-                           : dst.[i].
-
-(* map *)
-op map: ('x -> 'y) -> 'x array -> 'y array.
-
-axiom length_map (xs:'x array) (f:'x -> 'y):
-  length (map f xs) = length xs.
-
-axiom get_map (xs:'x array) (f:'x -> 'y, i:int):
-  0 <= i < length(xs) =>
-  (map f xs).[i] = f (xs.[i]).
-
-(* map2 *) (* Useful for bitwise operations *)
-op map2: ('x -> 'y -> 'z) -> 'x array -> 'y array -> 'z array.
-
-axiom length_map2 (xs:'x array) (ys:'y array) (f:'x -> 'y -> 'z):
-  length xs = length ys =>
-  length (map2 f xs ys) = length xs.
-
-axiom get_map2 (xs:'x array) (ys:'y array) (f:'x -> 'y -> 'z, i:int):
-  length xs = length ys =>
-  0 <= i < length xs =>
-  (map2 f xs ys).[i] = f (xs.[i]) (ys.[i]).
-
-(* mapi *)
-op mapi: (int -> 'x -> 'y) -> 'x array -> 'y array.
-
-axiom length_mapi (f:int -> 'x -> 'y) (xs:'x array):
-  length (mapi f xs) = length xs.
-
-axiom get_mapi (f:int -> 'x -> 'y) (xs:'x array) (i:int):
-  0 <= i < length xs =>
-  (mapi f xs).[i] = f i (xs.[i]).
-
-(* fold_left *)
-op fold_left: ('state -> 'x -> 'state) -> 'state -> 'x array -> 'state.
-
-axiom fold_left_empty (f:'state -> 'x -> 'state) s:
-  (fold_left f s empty) = s.
-
-axiom fold_left_cons (f:'state -> 'x -> 'state) s xs:
-  0 < length xs =>
-  (fold_left f s xs) = f (fold_left f s (sub xs 1 (length xs - 1))) xs.[0].
-
-(* fold_right *)
-op fold_right: ('state -> 'x -> 'state) -> 'state -> 'x array -> 'state.
-
-axiom fold_right_empty xs (f:'state -> 'x -> 'state) s:
-  length xs = 0 =>
-  (fold_right f s xs) = s.
-
-axiom fold_right_cons (f:'state -> 'x -> 'state) s xs:
-  0 < length xs =>
-  (fold_right f s xs) = fold_right f (f s xs.[0]) (sub xs 1 (length xs - 1)).
-
-(* lemmas *)
-lemma empty_append_l (xs:'x array):
-  (xs || empty) = xs.
-proof strict.
-apply array_ext; split.
-  by rewrite length_append length_empty.
-  by intros=> i; rewrite length_append length_empty /= => i_bnd;
-     rewrite get_append ?length_append ?length_empty /= // i_bnd.
-qed.
-
-lemma empty_append_r (xs:'x array):
-  (empty || xs) = xs.
-proof strict.
-apply array_ext; split.
-  by rewrite length_append length_empty.
-  by intros=> i; rewrite length_append length_empty /= => i_bnd;
-     rewrite get_append ?length_append ?length_empty /= //;
-     cut ->: (0 <= i < 0) = false by smt.
-qed.
-
-lemma sub_cons x (xs:'x array):
-  sub (x::xs) 1 (length (x::xs) - 1) = xs.
-proof strict.
-apply array_ext; smt.
-qed.
-
-lemma sub_full (xs:'x array):
-  sub xs 0 (length xs) = xs.
-proof strict.
-apply array_ext; split.
-  by rewrite length_sub; first 2 smt.
-  by intros=> i; rewrite length_sub //=; first 2 smt.
-qed.
-
-lemma sub_append_l (xs0 xs1:'x array):
-  sub (xs0 || xs1) 0 (length xs0) = xs0.
-proof strict.
-by apply array_ext; split; smt.
-qed.
-
-lemma sub_append_r (xs0 xs1:'x array):
-  sub (xs0 || xs1) (length xs0) (length xs1) = xs1.
-proof strict.
-by apply array_ext; split; smt.
-qed.
-
-lemma sub_append_sub (xs:'x array) (i l1 l2:int):
-  0 <= i => 0 <= l1 => 0 <= l2 => i + l1 + l2 <= length xs =>
-  (sub xs i l1 || sub xs (i + l1) l2) = sub xs i (l1 + l2).
-proof strict.
-by intros=> i_pos l1_pos l2_pos i_l1_l2_bnd;
-   apply array_ext; split; smt.
-qed.
-
-lemma map_map (f:'x -> 'y) (g:'y -> 'z) xs:
- map g (map f xs) = map (fun x, g (f x)) xs.
-proof strict.
-apply array_ext; split.
-  by rewrite !length_map.
-  by intros=> i; rewrite !length_map=> i_bnd;
-     rewrite !get_map ?length_map.
-qed.
-
-lemma map_cons (f:'x -> 'y) x xs:
-  map f (x::xs) = (f x)::(map f xs).
-proof strict.
-apply array_ext; split; smt.
-qed.
-
-lemma mapi_mapi (f:int -> 'x -> 'y) (g:int -> 'y -> 'z) xs:
- mapi g (mapi f xs) = mapi (fun k x, g k (f k x)) xs.
-proof strict.
-apply array_ext; split.
-  by rewrite !length_mapi.
-  by intros=> i; rewrite !length_mapi=> i_bnd; rewrite ?get_mapi ?length_mapi.
-qed.
-
-lemma mapi_id (f:int -> 'x -> 'x) (xs:'x array):
- (forall k x, 0 <= k < length xs => f k x = x) =>
- mapi f xs = xs.
-proof strict.
-intros=> f_id; apply array_ext; split.
-  by rewrite length_mapi.
-  by intros=> i; rewrite !length_mapi=> i_bnd; rewrite ?get_mapi ?length_mapi ?f_id.
-qed.
-
-(* Useless? *)
-lemma fold_left_deterministic: forall (f1 f2:'state -> 'x -> 'state) s1 s2 xs1 xs2,
-  f1 = f2 => s1 = s2 => xs1 = xs2 =>
-  fold_left f1 s1 xs1 = fold_left f2 s2 xs2
-by [].
-
-lemma fold_right_map (f:'x -> 'y -> 'x) (x:'x) (g:'z -> 'y) (zs:'z array):
- fold_right f x (map g zs) = fold_right (fun x y, f x (g y)) x zs.
-proof strict.
- elim/array_ind zs x.
-  by intros=> x; rewrite !fold_right_empty ?length_map ?length_empty.
-  intros=> z zs IH x; rewrite !(fold_right_cons _ x); first 2 smt.
-  by rewrite map_cons !sub_cons IH 2?get_cons; first 2 smt.
-qed.
-
-(* Alternative induction principle: building arrays from the back *)
-lemma array_ind_snoc (p:'x array -> bool):
-  p empty =>
-  (forall x xs, p xs => p (xs:::x)) =>
-  (forall xs, p xs).
-proof strict.
-intros=> p0 prec xs.
-cut h : (forall n, 0 <= n => forall xs, length xs = n => p xs).
-  elim => //; first smt.
-  intros=> i ipos hrec xs' hlen.
-  cut ->: xs' = (sub xs' 0 i):::xs'.[i] by (apply array_ext; smt).
-  apply prec.
-  apply hrec.  
-  by rewrite length_sub; smt.
-by apply (h (length xs) _);smt.
-qed.
-
-(* This proof needs cleaned up, and the lemma library completed. *)
-lemma fold_length (xs:'x array):
-  fold_left (fun n x, n + 1) 0 xs = length xs.
-proof strict.
-elim/array_ind xs.
-  by rewrite fold_left_empty length_empty.
-  by intros=> x xs IH; rewrite fold_left_cons;
-       [ | cut ->: sub (x::xs) 1 (length (x::xs) - 1) = xs by (apply array_ext; smt)];
-     smt.
-qed.
-
-lemma blit_append (dst src:'x array):
-  length src <= length dst =>
-  blit dst 0 src 0 (length src) = (src || (sub dst (length src) (length dst - length src))).
-proof strict.
-intros=> src_dst; apply array_ext; split; smt.
-qed.
-
-(** Things that are not in the OCaml array library:
-      - take and drop (prefix and suffix),
-      - complex initialization,
-      - logical predicates *)
-(* take *)
-op take (len:int) (xs:'a array) = sub xs 0 len.
-
-lemma length_take (xs:'a array) (l:int):
-  0 <= l <= length xs =>
-  length (take l xs) = l
-by smt.
-
-lemma get_take (xs:'a array) (l k:int):
-  0 <= k < l <= length xs =>
-  (take l xs).[k] = xs.[k]
-by smt.
-
-(* drop *)
-op drop (len:int) (xs:'a array) = sub xs len (length xs-len).
-
-lemma length_drop (xs:'a array) (l:int):
-  0 <= l <= length xs =>
-  length (drop l xs) = length xs - l
-by smt.
-
-lemma get_drop  (xs:'a array) (l k:int):
-  0 <= l => 0 <= k < length xs-l =>
-  (drop l xs).[k] = xs.[l + k]
-by smt.
-
-lemma take_drop (xs:'a array) (l:int):
-  0 <= l <= length xs =>
-  (take l xs || drop l xs) = xs
-by smt full.
-
-(* init_dep: init, but using a function that may depend
-   on the rest of the array! *)
-op init_dep: 'x array -> int -> (int -> 'x array -> 'x) -> 'x array.
-
-axiom init_dep_def (xs:'x array) (size:int) (f:int -> 'x array -> 'x):
-  init_dep xs size f =
-    let r = make (length xs + size) xs.[0] in (* creates the space *)
-    let r = blit r 0 xs 0 (length xs) in      (* copies the initial value in *)
-    iteri size (fun i r => r.[i + length xs <- f i r]) r.
-
-(* all: this is computable because all arrays are finite *)
-op all: ('x -> bool) -> 'x array -> bool.
-
-axiom all_def p (xs:'x array):
-  all p xs <=>
-  (forall i, 0 <= i < length xs => p xs.[i]).
-
-(* alli *)
-op alli: (int -> 'x -> bool) -> 'x array -> bool.
-
-axiom alli_def p (xs:'x array):
-  alli p xs <=>
-  (forall i, 0 <= i < length xs => p i xs.[i]).
-
-lemma alli_base p: alli p empty<:'x>.
-proof strict.
-by rewrite alli_def length_empty; smt.
-qed.
-
-lemma alli_ind p (x:'x) xs:
-  alli p (x::xs) =
-    (p 0 x /\ alli (fun i x, p (i + 1) x) xs).
-proof strict.
-rewrite (alli_def _ xs).
-cut ->: (p 0 x /\ forall (i:int), 0 <= i < length xs => (fun i x, p (i + 1) x) i xs.[i]) <=>
-         forall (i:int), 0 <= i < length (x::xs) => p i (x::xs).[i].
-  split; first smt.
-  intros=> alli; split.
-    cut ->: x = (x::xs).[0] by rewrite get_cons //=; smt.
-    by apply alli; first smt.
-  intros=> i i_bnd //=.
-  cut ->: xs.[i] = (x::xs).[i + 1] by rewrite get_cons //=; smt.
-  by apply alli; first smt.
-by rewrite -alli_def.
-qed.
-
-lemma alli_true p (xs:'x array):
-  (forall i x, p i x) =>
-  alli p xs.
-proof strict.
-by rewrite alli_def=> p_true i i_bnd;
-   apply p_true.
-qed.
-
-(* TODO *)
-
-(** Distribution on 'a array of length k from distribution on 'a *)
-(* We return the empty array when the length is negative *)
-theory Darray.
-  require import Distr.
-  require import Real.
-
-  op darray: int -> 'a distr -> 'a array distr.
-
-  (* Negative length case... This appears to be a necessary evil for now *)
-  (* At least it's only one axiom *)
-  axiom mu_neg (len:int) (d:'a distr) (p:'a array -> bool):
-    len < 0 =>
-    mu (darray len d) p = charfun p empty.
-
-  lemma mu_x (len:int) (d:'a distr) (x:'a array):
-    len < 0 =>
-    mu_x (darray len d) x = if x = empty then 1%r else 0%r.
-  proof strict.
-  rewrite /mu_x=> len_neg; case (x = empty).
-    by intros=> ->; rewrite mu_neg.
-    by rewrite mu_neg// /charfun pred1E=> ->.
-  qed.
-
-  lemma supp_neg (len:int) (d:'a distr) (x:'a array):
-    len < 0 =>
-    in_supp x (darray len d) <=> x = empty
-  by [].
-
-  lemma weight_neg (len:int) (d:'a distr):
-    len < 0 =>
-    weight (darray len d) = 1%r
-  by [].
-
-  (* Non-negative length case *)
-  axiom mu_x_def (len: int) (d:'a distr) (x:'a array):
-    len = length x =>
-    mu_x (darray len d) x = fold_right (fun p x, p * mu_x d x) 1%r x.
-
-  axiom supp_def (len:int) (x:'a array) (d:'a distr):
-    0 <= len =>
-    in_supp x (darray len d) <=>
-    (length x = len /\ all (support d) x).
-
-  lemma supp_full (len:int) (d:'a distr) (x:'a array):
-    0 <= len =>
-    (forall y, in_supp y d) =>
-    length x = len <=> in_supp x (darray len d).
-  proof strict.
-  intros leq0_len dF; split.
-    by intros=> Hlen; rewrite Darray.supp_def=> //; split=> //;
-       rewrite all_def=> i Hi; rewrite /support dF.
-    by rewrite Darray.supp_def.
-  qed.
-
-  lemma supp_len (len:int) (x: 'a array) (d:'a distr):
-    0 <= len =>
-    in_supp x (darray len d) => length x = len.
-  proof strict. by intros=> leq0_len; rewrite supp_def. qed.
-
-  lemma supp_k (len:int) (x: 'a array) (d:'a distr) (k:int):
-    0 <= k < len =>
-    in_supp x (darray len d) =>
-    in_supp x.[k] d.
-  proof strict.
-  intros=> k_bnd; rewrite supp_def -/(support d x.[k]); first smt.
-  by intros=> [len_def all_in_supp]; subst;
-     generalize all_in_supp; rewrite all_def=> H; apply H.
-  qed.
-
-  (* This would be a lemma by definition of ^
-     if we had it in the correct form (if we know that Real is a field) *)
-  axiom weight_d (d:'a distr) len:
-    0 <= len => weight (darray len d) = (weight d) ^ len.
-
-  lemma darrayL (d:'a distr) len:
-    0 <= len =>
-    weight d = 1%r =>
-    weight (darray len d) = 1%r.
-  proof strict.
-  intros leq0_len H; rewrite (weight_d d len) // H.
-  smt full.
-  qed.
-
-  (* if len is negative, then uniformity is easy to prove.
-     otherwise, the folded function can be replaced with the same constant for x and y
-     (but we need to know that it is only applied to elements of d's support,
-      which justifies leaving it as an axiom for now) *)
-  axiom uniform (d:'a distr) len:
-    is_uniform d =>
-    is_uniform (darray len d).
-end Darray.
